src/ast_instructions.v
@@ -25,13 +25,13 @@ Inductive instr_sig {T : Type} :=
 
 
 (* thoses are the type and lemmas that have to be implemented by the user *)
-(*
+
 Variable tag : Type.
 Variable beq_T : tag -> tag -> bool.
 Variable beq_T_refl : forall (t : tag), beq_T t t = true.
 Variable beq_T_rev : forall (t1 t2 : tag), beq_T t1 t2 = true <-> t1 = t2.
-*)
 
+(*
 (* need an implementation to compile *)
 Inductive tag :=
 | bidon1 : tag
@@ -61,7 +61,7 @@ Proof.
   intros. case t1; case t2; split; try auto; try discriminate.
 Qed.
 (* end of dummy implementation *)
-
+*)
 Scheme Equality for list.
 
 Definition instr_sig_beq (T : Type) (i1 i2 : instr_sig) :=
